End of Curve Code

specs/Hacl.P256.PointDouble.fst
@@ -99,3 +99,26 @@ let point_double x_out y_out z_out x_in y_in z_in =
   felem_reduce_zero105 y_out tmp
 )
   
+
+val point_double_small:
+  x_out:smallfelem -> y_out:smallfelem -> z_out:smallfelem ->
+  x_in:smallfelem -> y_in:smallfelem -> z_in:smallfelem -> Stack unit
+    (requires (fun h -> True))
+    (ensures (fun h0 _ h1 -> True))
+
+let point_double_small x_out y_out z_out x_in y_in z_in =
+	alloc  #(uint_t U128) #(unit) #(v(size 24)) (size 24) (u128(0)) 
+		[BufItem x_in; BufItem y_in; BufItem z_in] [BufItem x_out; BufItem y_out; BufItem z_out] 
+    (fun h0 _ h1 -> True) (
+      fun temp ->
+		let felem_x_out = sub temp (size 0) (size 4) in
+		let felem_y_out = sub temp (size 4) (size 4) in
+		let felem_z_out = sub temp (size 8) (size 4) in
+		let felem_x_in = sub temp (size 12) (size 4) in
+		let felem_y_in = sub temp (size 16) (size 4) in
+		let felem_z_in = sub temp (size 20) (size 4) in
+  point_double felem_x_out felem_y_out felem_z_out felem_x_in felem_y_in felem_z_in;
+  felem_shrink x_out felem_x_out;
+  felem_shrink y_out felem_y_out;
+  felem_shrink z_out felem_z_out
+)
