specs/Hacl.P256.Copy.fst
@@ -1,0 +1,61 @@
+module Hacl.P256.Copy
+
+open FStar.Mul
+
+open FStar.HyperStack
+open FStar.HyperStack.ST
+
+open Spec.Lib.Loops
+
+open Spec.Lib
+open Spec.Lib.IntSeq
+
+open Spec.Lib.IntTypes
+open Spec.Lib.IntBuf
+
+open Spec.Lib.IntSeq.Lemmas
+open Spec.Lib.IntBuf.Lemmas
+
+open P256.S
+open Hacl.P256.Zeros
+open Hacl.P256.Shrink
+
+open Hacl.P256.Mult
+open Hacl.P256.Reduce
+open Hacl.P256.Square
+open Hacl.P256.Contract
+open Hacl.P256.SmallNegation
+
+
+val copy_conditional:
+  out:felem -> input:felem -> mask:limb -> Stack unit
+    (requires (fun h -> True))
+    (ensures (fun h0 _ h1 -> True))
+
+let copy_conditional out input mask =
+  let inv (h1:mem) (i:nat) = True in
+  let f (i:size_t) : Stack unit
+    (requires (fun h -> True))
+    (ensures (fun h0 _ h1 -> True))
+    = let inputi = input.(i) in
+      let outi = out.(i) in
+      let tmp = mask &. (inputi ^. outi) in
+      out.(i) <- outi ^. tmp in
+  for (size 0) (size 4) inv f
+
+val copy_small_conditional:
+  out:felem -> input:smallfelem -> mask:limb -> Stack unit
+    (requires (fun h -> True))
+    (ensures (fun h0 _ h1 -> True))
+
+let copy_small_conditional out input mask =
+  let mask64 = to_u64(mask) in
+  let inv (h1:mem) (i:nat) = True in
+  let f (i:size_t) : Stack unit
+    (requires (fun h -> True))
+    (ensures (fun h0 _ h1 -> True))
+    = let inputi = input.(i) in
+      let outi = out.(i) in
+      let tmp = to_u128 (to_u64(inputi &. mask64)) |. (outi &. lognot mask) in
+      out.(i) <- tmp in
+  for (size 0) (size 4) inv f
