specs/Hacl.P256.PointAdd.fst
@@ -1,0 +1,200 @@
+module Hacl.P256.PointAdd
+
+open FStar.Mul
+
+open FStar.HyperStack
+open FStar.HyperStack.ST
+
+open Spec.Lib.Loops
+
+open Spec.Lib
+open Spec.Lib.IntSeq
+
+open Spec.Lib.IntTypes
+open Spec.Lib.IntBuf
+
+open Spec.Lib.IntSeq.Lemmas
+open Spec.Lib.IntBuf.Lemmas
+
+open P256.S
+open Hacl.P256.Zeros
+open Hacl.P256.Shrink
+
+open Hacl.P256.Mult
+open Hacl.P256.Reduce
+open Hacl.P256.Square
+open Hacl.P256.Contract
+open Hacl.P256.SmallNegation
+open Hacl.P256.IsZero
+open Hacl.P256.PointDouble
+open Hacl.P256.Copy
+
+val point_add:
+  x3:felem -> y3:felem -> z3:felem ->
+  x1:felem -> y1:felem -> z1:felem ->
+  mixed:(uint_t U32) -> 
+  x2:smallfelem -> y2:smallfelem -> z2:smallfelem ->
+  Stack unit
+    (requires (fun h -> True))
+    (ensures (fun h0 _ h1 -> True))
+
+let point_add x3 y3 z3 x1 y1 z1 mixed x2 y2 z2 =
+	alloc  #(uint_t U128) #(unit) #(v(size 52)) (size 52) (u128(0)) 
+		[BufItem x1; BufItem y1; BufItem z1;
+			BufItem x2; BufItem y2; BufItem z2] 
+		[BufItem x3; BufItem y3; BufItem z3] 
+    (fun h0 _ h1 -> True) (
+      fun temp ->
+  let ftmp =  sub temp (size 0) (size 4) in
+  let ftmp2 = sub temp (size 4) (size 4) in
+  let ftmp3 = sub temp (size 8) (size 4) in
+  let ftmp4 =  sub temp (size 12) (size 4) in
+  let ftmp5 =  sub temp (size 16) (size 4) in
+  let ftmp6 =  sub temp (size 20) (size 4) in
+  let x_out =  sub temp (size 24) (size 4) in
+  let y_out =  sub temp (size 28) (size 4) in
+  let z_out =  sub temp (size 32) (size 4) in
+  let tmp   =  sub temp (size 36) (size 8) in 
+  let tmp2   = sub temp (size 44) (size 8) in 
+  let small1 = create_smallfelem() in
+  let small2 = create_smallfelem() in
+  let small3 = create_smallfelem() in
+  let small4 = create_smallfelem() in
+  let small5 = create_smallfelem() in
+
+  felem_shrink small3 z1;
+
+  let z1_is_zero = smallfelem_is_zero small3 in
+  let z2_is_zero = smallfelem_is_zero z2 in
+
+  smallfelem_square tmp small3;
+  felem_reduce ftmp tmp;
+  felem_shrink small1 ftmp;
+
+  if (mixed = u32(0)) then
+    begin
+      smallfelem_square tmp z2;
+      felem_reduce ftmp2 tmp;
+      felem_shrink small2 ftmp2;
+
+      felem_shrink small5 x1;
+
+      smallfelem_mul tmp small5 small2;
+      felem_reduce ftmp3 tmp;
+
+      felem_assign ftmp5 z1;
+      felem_small_sum ftmp5 z2;
+
+      felem_square tmp ftmp5;
+      felem_reduce ftmp5 tmp;
+      felem_sum ftmp2 ftmp;
+      felem_diff ftmp5 ftmp2;
+
+      smallfelem_mul tmp small2 z2;
+      felem_reduce ftmp2 tmp;
+
+      felem_mul tmp y1 ftmp2;
+      felem_reduce ftmp6 tmp
+    end
+  else
+    begin
+      felem_assign ftmp3 x1;
+
+      felem_assign ftmp5 z1;
+      felem_scalar ftmp5 (u32 1);
+
+      felem_assign ftmp6 y1
+    end;
+
+  smallfelem_mul tmp x2 small1;
+  felem_reduce ftmp4 tmp;
+
+  felem_diff_zero107 ftmp4 ftmp3;
+  felem_shrink small4 ftmp4;
+
+  let x_equal = smallfelem_is_zero small4 in
+
+  felem_small_mul tmp small4 ftmp5;
+  felem_reduce z_out tmp;
+
+  smallfelem_mul tmp small1 small3;
+  felem_reduce ftmp tmp;
+
+  felem_small_mul tmp y2 ftmp;
+  felem_reduce ftmp5 tmp;
+
+  felem_diff_zero107 ftmp5 ftmp6;
+  felem_scalar ftmp5 (u32 1);
+  felem_shrink small1 ftmp5;
+  let y_equal = smallfelem_is_zero small1 in
+
+  let zero = u128(0) in
+  if  ((x_equal <> zero) && (y_equal <> zero) && not(z1_is_zero <> zero) && not(z2_is_zero <> zero)) then
+      begin
+        point_double x3 y3 z3 x1 y1 z1
+      end
+  else
+      begin
+        felem_assign ftmp ftmp4;
+        felem_scalar ftmp (u32 1);
+        felem_square tmp ftmp;
+        felem_reduce ftmp tmp;
+        felem_mul tmp ftmp4 ftmp;
+        felem_reduce ftmp2 tmp;
+        felem_mul tmp ftmp3 ftmp;
+        felem_reduce ftmp4 tmp;
+        smallfelem_square tmp small1;
+        felem_reduce x_out tmp;
+        felem_assign ftmp3 ftmp4;
+        felem_scalar ftmp4 (u32 1);
+        felem_sum ftmp4 ftmp2;
+        felem_diff x_out ftmp4;
+
+        felem_diff_zero107 ftmp3 x_out;
+        felem_small_mul tmp small1 ftmp3;
+        felem_mul tmp2 ftmp6 ftmp2;
+        longfelem_scalar tmp2 (u64 1);
+        longfelem_diff tmp tmp2;
+        felem_reduce_zero105 y_out tmp;
+
+        copy_small_conditional x_out x2 z1_is_zero;
+        copy_conditional x_out x1 z2_is_zero;
+        copy_small_conditional y_out y2 z1_is_zero;
+        copy_conditional y_out y1 z2_is_zero;
+        copy_small_conditional z_out z2 z1_is_zero;
+        copy_conditional z_out z1 z2_is_zero;
+        felem_assign x3 x_out;
+        felem_assign y3 y_out;
+        felem_assign z3 z_out
+      end
+  )
+
+
+val point_add_small:
+  x3:smallfelem -> y3:smallfelem -> z3:smallfelem ->
+  x1:smallfelem -> y1:smallfelem -> z1:smallfelem ->
+  x2:smallfelem -> y2:smallfelem -> z2:smallfelem -> Stack unit
+    (requires (fun h -> True))
+    (ensures (fun h0 _ h1 -> True))
+
+let point_add_small x3 y3 z3 x1 y1 z1 x2 y2 z2 =
+	alloc  #(uint_t U128) #(unit) #(v(size 24)) (size 24) (u128(0)) 
+		[BufItem x1; BufItem y1; BufItem z1;
+			BufItem x2; BufItem y2; BufItem z2] 
+		[BufItem x3; BufItem y3; BufItem z3] 
+    (fun h0 _ h1 -> True) (
+      fun temp ->
+  let felem_x3 = sub temp (size 0) (size 4) in
+  let felem_y3 = sub temp (size 4) (size 4) in
+  let felem_z3 = sub temp (size 8) (size 4) in
+  let felem_x1 = sub temp (size 12) (size 4) in
+  let felem_y1 = sub temp (size 16) (size 4) in
+  let felem_z1 = sub temp (size 20) (size 4) in
+  smallfelem_expand felem_x1 x1;
+  smallfelem_expand felem_y1 y1;
+  smallfelem_expand felem_z1 z1;
+  point_add felem_x3 felem_y3 felem_z3 felem_x1 felem_y1 felem_z1 (u32 0) x2 y2 z2;
+  felem_shrink x3 felem_x3;
+  felem_shrink y3 felem_y3;
+  felem_shrink z3 felem_z3
+)
